\documentclass[12pt]{article}
\linespread{1.25}

\begin{document}

$\frac{-7}{37}x + \frac{12}{27} = \frac{10}{22}x + \frac{1}{42}$\\
$\frac{-2}{45}x + \frac{-14}{1} = \frac{16}{30}x + \frac{-7}{37}$\\
$\frac{-1}{1}x + \frac{-14}{7} = \frac{20}{14}x + \frac{-18}{13}$\\
$\frac{0}{12}x + \frac{-17}{23} = \frac{-3}{36}x + \frac{-1}{26}$\\
$\frac{13}{28}x + \frac{-19}{15} = \frac{17}{28}x + \frac{-9}{6}$\\
$\frac{20}{37}x + \frac{16}{28} = \frac{-16}{7}x + \frac{15}{28}$\\
$\frac{-7}{13}x + \frac{2}{14} = \frac{-12}{2}x + \frac{-17}{7}$\\
$\frac{6}{29}x + \frac{12}{1} = \frac{16}{28}x + \frac{-12}{24}$\\
$\frac{3}{10}x + \frac{2}{41} = \frac{19}{48}x + \frac{11}{38}$\\
$\frac{8}{1}x + \frac{9}{20} = \frac{-3}{26}x + \frac{-11}{5}$\\
$\frac{17}{43}x + \frac{-10}{29} = \frac{-2}{8}x + \frac{3}{49}$\\
$\frac{3}{19}x + \frac{5}{29} = \frac{-5}{49}x + \frac{-13}{7}$\\
$\frac{7}{45}x + \frac{-11}{19} = \frac{-3}{22}x + \frac{15}{48}$\\
$\frac{-2}{15}x + \frac{-6}{13} = \frac{-8}{35}x + \frac{-7}{24}$\\
$\frac{7}{3}x + \frac{10}{27} = \frac{-10}{31}x + \frac{-4}{33}$\\
$\frac{-3}{1}x + \frac{17}{21} = \frac{-8}{4}x + \frac{3}{3}$\\
$\frac{13}{13}x + \frac{-9}{2} = \frac{-17}{48}x + \frac{-2}{34}$\\
$\frac{0}{12}x + \frac{-16}{12} = \frac{-5}{41}x + \frac{13}{15}$\\
$\frac{-10}{49}x + \frac{1}{22} = \frac{13}{13}x + \frac{9}{49}$\\
$\frac{7}{43}x + \frac{-10}{40} = \frac{-16}{9}x + \frac{9}{43}$\\

\end{document}